\documentclass{article}
\usepackage[utf8]{inputenc}
\usepackage{amsmath}
\usepackage[margin=1cm]{geometry}
\newcommand{\given}{\, | \,}
\begin{document}
	$\bullet$ Sequential logistic regression model for $\left\{
	\begin{array}{lll}
		\eta_i = 1 & \text{or} & \eta_i > 1\\
		\eta_i = 2 & \text{or}& \eta_i > 2 \\
		\eta_i = 3 & \text{or}& \eta_i = 4 \\
	\end{array}
	\right.$ 
	to replace proportional odds model for $\eta_i$:
	\\ 
	\\
	$\left\{
	\begin{array}{l}
		\text{logit}  \ P(\eta_i = 1 \given x_i,\alpha_{1}, \beta_{1}) = \alpha_{1} - x_i^T \beta_{1} \\
		\\
		\text{logit}  \ P(\eta_i = 2 \given \eta_i \geq 2,x_i, \alpha_{2}, \beta_{2}) = \alpha_{2} - x_i^T \beta_{2} \\
		\\
		\text{logit}  \ P(\eta_i = 3 \given \eta_i \geq 3,x_i, \alpha_{3}, \beta_{3}) =  \alpha_{3} - x_i^T \beta_{3} \\
	\end{array}
	\right.$ 	\\
	\\
	\\
	$\Rightarrow$ Likelihood:
	\\
	\\
	$P(\eta_i = 1 \given x_i, \alpha_1,\beta_1) = \frac{exp(\alpha_1 - x_i^T \beta_{1})}{1+exp(\alpha_1 - x_i^T \beta_{1})}$ 
\begin{flalign*}
		P(\eta_i = 2 \given x_i, \alpha_{1,2}, \beta_{1,2}) 
		&= P(\eta_i > 1 \given  x_i, \alpha_1,\beta_1)P(\eta_i = 2 \given \eta_i > 1, x_i, \alpha_2,\beta_2)  &\\
		&= (1-P(\eta_i = 1 \given ...))(P(\eta_i = 2 \given \eta_i > 1,...)) &\\
		&=\frac{1}{1+exp(\alpha_1 - x_i^T \beta_{1})} \frac{exp(\alpha_2 - x_i^T \beta_{2})}{1+exp(\alpha_2 - x_i^T \beta_{2})}
\end{flalign*}
\begin{flalign*}
	P(\eta_i = 3 \given x_i, \alpha_{1,2,3}, \beta_{1,2,3}) 
	&= P(\eta_i > 1 \given  x_i, \alpha_1,\beta_1)P(\eta_i > 2 \given \eta_i > 1, x_i, \alpha_2,\beta_2)P(\eta_i = 3 \given \eta_i > 2, x_i, \alpha_3,\beta_3)   &\\
	&= (1-P(\eta_i = 1 \given ...))(1-P(\eta_i = 2 \given \eta_i > 1,...)) P(\eta_i = 3 \given \eta_i > 2,...)&\\
	&=\frac{1}{1+exp(\alpha_1 - x_i^T \beta_{1})} 
	\frac{1}{1+exp(\alpha_2 - x_i^T \beta_{2})}
	\frac{exp(\alpha_3 - x_i^T \beta_{3})}{1+exp(\alpha_3 - x_i^T \beta_{3})}
\end{flalign*}

\begin{flalign*}
	P(\eta_i = 4 \given x_i, \alpha_{1,2,3}, \beta_{1,2,3}) 
	&= 1- P(\eta_i = 1 \given x_i, \alpha_{1}, \beta_{1}) -P(\eta_i = 2 \given x_i, \alpha_{2}, \beta_{2}) -P(\eta_i = 3 \given x_i, \alpha_{3}, \beta_{3}) &\\
	&=1- \frac{exp(\alpha_1 - x_i^T \beta_{1})}{1+exp(\alpha_1 - x_i^T \beta_{1})} - \frac{1}{1+exp(\alpha_1 - x_i^T \beta_{1})} \frac{exp(\alpha_2 - x_i^T \beta_{2})}{1+exp(\alpha_2 - x_i^T \beta_{2})} &\\
	& - \frac{1}{1+exp(\alpha_1 - x_i^T \beta_{1})} 
	\frac{1}{1+exp(\alpha_2 - x_i^T \beta_{2})}
	\frac{exp(\alpha_3 - x_i^T \beta_{3})}{1+exp(\alpha_3 - x_i^T \beta_{3})} &\\
	&=\frac{1}{1+exp(\alpha_1 - x_i^T \beta_{1})} - \frac{1}{1+exp(\alpha_1 - x_i^T \beta_{1})} \frac{exp(\alpha_2 - x_i^T \beta_{2})}{1+exp(\alpha_2 - x_i^T \beta_{2})} &\\
	&- \frac{1}{1+exp(\alpha_1 - x_i^T \beta_{1})} 
	\frac{1}{1+exp(\alpha_2 - x_i^T \beta_{2})}
	\frac{exp(\alpha_3 - x_i^T \beta_{3})}{1+exp(\alpha_3 - x_i^T \beta_{3})} 
\end{flalign*}
%	$P(\eta_i = 4 \given x_i, \alpha_{1,2,3},\beta_{1,2,3}) = 
%	[1-P(\eta_i = 1 \given \eta_i \geq 1, x_i, \alpha_{1}, \beta_{1})]  
%	[1-P(\eta_i = 2 \given \eta_i \geq 2,x_i, \alpha_{2},	\beta_{2})] 
%	[1-P(\eta_i = 3 \given \eta_i \geq 3,x_i, \alpha_{3},\beta_{3})]$
\\


$\bullet$ Conditional model for $pgg_i \given \eta_i = j, z_i, \gamma_j$ 
\\
\\
$\text{logit} \ P(pgg_i = j \given \eta_i = j, z_i, \gamma_1) = z_i^T \gamma_1$
\\
\\
$\text{logit} \ P( |pgg_i - \eta_i| = 1 \given \eta_i = j, z_i, \gamma_2)= z_i^T \gamma_2$
\\
\\
$\text{logit} \ P( |pgg_i - \eta_i| = 2 \given \eta_i = j, z_i, \gamma_3)= z_i^T \gamma_3$ if needed
\\

Example: for $j = 3$
\\
$\text{logit} \ P(pgg_i = 3 \given \eta_i = 3, z_i, \gamma_1) = z_i^T \gamma_1$
\\
\\
$\text{logit} \ P( pgg_i =1  \given \eta_i = 3, z_i, \gamma_2)= z_i^T \gamma_2$
\\
\\
$\ P( pgg_i = 2  \text{ or } 4 \given \eta_i = 3, z_i, \gamma_1, \gamma_2)= [1-P(pgg_i = 3 \given \eta_i = 3,z_i, \gamma_1)][1-P(pgg_i = 1 \given \eta_i = 3,z_i, \gamma_2)]$
\\

\end{document}